iris/BootShared.v
@@ -1432,7 +1432,8 @@ Section BootAlloc.
     iMod (disk_ghosts_alloc gen_id (g.(gdev).(dvirtio))
             ltac:(rewrite Hv0; apply virtio_reset_not_live)
             ltac:(rewrite Hv0; apply virtio_reset_seen)
-            ltac:(rewrite Hv0; apply virtio_reset_used_idx))
+            ltac:(rewrite Hv0; apply virtio_reset_used_idx)
+            ltac:(rewrite Hv0; apply virtio_reset_landed))
       as (γv) "(%Himg & Hproto & Hcfg & Hclaim & #Hdone & Hpbody)".
     iMod (dev_inv_alloc ⊤ γd γv
             with "[Huf Hpf Hvf Hacc Hout Htxa Hdla Hproto] Hpbody")
