iris/ProofVirtioDiskRwE.v
@@ -227,13 +227,13 @@ Section ProofVirtioDiskRwE.
       (pd pav pu : SailStdpp.Values.mword 64) (K : nat) (eb : bool)
       (sp0 b : Arch.pa) (wr sector : SailStdpp.Values.mword 64)
       (bs_buf bs_disk : list (bv 8)) (m0 : regfile)
-      (kq : nat * positive) (lks : gset string) : iProp Σ :=
+      (kq : nat * positive) (ks : list (nat * positive)) (lks : gset string) : iProp Σ :=
     (wp_next (CID0 := CID0) true (proc_addr j) (fun (CID : CpuId) =>
      ∀ (M : regfile) (q np nr : nat) (fl pk : gmap nat dclaim)
        (tr : gmap nat (nat * nat * nat)) (fr : nat -> bool) (h m2 t : nat) pin,
        ⌜vdrw_regs M sp0 b wr sector /\ vdrw_hi M m0⌝ -∗
        ⌜tri_ok (h, m2, t)⌝ -∗
-       ⌜pk !! q = Some (DClaim b (vdrwd_slot kq b h wr sector
+       ⌜pk !! q = Some (DClaim b (vdrwd_slot kq ks b h wr sector
                                     (vdrwd_sldata wr bs_buf bs_disk))
                                (h, m2, t) pin)⌝ -∗
        ⌜pin ∖ range_map (d_ring pav (q `mod` 8)) 2
@@ -251,7 +251,7 @@ Section ProofVirtioDiskRwE.
        pc_is (mword_of_int (KernelSyms.virtio_disk_rw + 0x1d2) : mword 64) -∗
        locked γk cpu_id -∗
        vdrw_body γd pd pav np nr fl pk tr fr -∗
-       disk_claim γd q (DClaim b (vdrwd_slot kq b h wr sector
+       disk_claim γd q (DClaim b (vdrwd_slot kq ks b h wr sector
                                     (vdrwd_sldata wr bs_buf bs_disk))
                                (h, m2, t) pin) -∗
        vdrw_slot_rest m2 -∗ vdrw_slot_rest t -∗
@@ -267,7 +267,7 @@ Section ProofVirtioDiskRwE.
       (pd pav pu : SailStdpp.Values.mword 64) (K : nat) (eb : bool)
       (sp0 b : Arch.pa) (wr sector : SailStdpp.Values.mword 64)
       (bs_buf bs_disk : list (bv 8)) (h m2 t : nat) (q : nat) (pin : _)
-      (m0 : regfile) (kq : nat * positive) (lks : gset string) : iProp Σ :=
+      (m0 : regfile) (kq : nat * positive) (ks : list (nat * positive)) (lks : gset string) : iProp Σ :=
     (wp_next (CID0 := CID0) true (proc_addr j) (fun (CID : CpuId) =>
      ∀ M : regfile,
        ⌜vdrw_regs M sp0 b wr sector
@@ -281,7 +281,7 @@ Section ProofVirtioDiskRwE.
        pc_is (mword_of_int (KernelSyms.virtio_disk_rw + 0x1b4) : mword 64) -∗
        locked γk cpu_id -∗
        disk_res γd pd pav pu -∗
-       disk_claim γd q (DClaim b (vdrwd_slot kq b h wr sector
+       disk_claim γd q (DClaim b (vdrwd_slot kq ks b h wr sector
                                     (vdrwd_sldata wr bs_buf bs_disk))
                                (h, m2, t) pin) -∗
        vdrw_slot_rest m2 -∗ vdrw_slot_rest t -∗
@@ -296,7 +296,7 @@ Section ProofVirtioDiskRwE.
                             (vdrwd_bufwin b wr bs_buf))
         /\ pm_ok (vdrwd_pinr_regions pd b h m2 t wr sector
                     (vdrwd_bufwin b wr bs_buf))⌝ -∗
-       vdrw_p5_exit CID0 γk γs j γd pd pav pu K eb sp0 b wr sector bs_buf bs_disk m0 kq lks -∗
+       vdrw_p5_exit CID0 γk γs j γd pd pav pu K eb sp0 b wr sector bs_buf bs_disk m0 kq ks lks -∗
        WP (Loop : expr riscv_lang)))%I.
 
   (* ------------------------------------------------------------------- *)
@@ -369,7 +369,7 @@ Section ProofVirtioDiskRwE.
       (γu : uart_names) (γd : disk_names)
       (pd pav pu : SailStdpp.Values.mword 64) (K : nat) (eb : bool)
       (sp0 b : Arch.pa) (wr sector : SailStdpp.Values.mword 64)
-      (bs_buf bs_disk : list (bv 8)) (m0 : regfile) (kq : nat * positive)
+      (bs_buf bs_disk : list (bv 8)) (m0 : regfile) (kq : nat * positive) (ks : list (nat * positive))
       (lks : gset string) :
     (K_virtio_disk_rw <= K)%nat ->
     (j < NPROC)%nat -> γs !! j = Some γl ->
@@ -387,9 +387,9 @@ Section ProofVirtioDiskRwE.
     dev_inv γu γd -∗
     is_lock γk d_lock "virtio_disk"%string (disk_res γd pd pav pu) -∗
     vdrw_p5_exit CID γk γs j γd pd pav pu K eb sp0 b wr sector bs_buf bs_disk
-                 m0 kq lks -∗
+                 m0 kq ks lks -∗
     P4.vdrw_p4_exit CID γk γs j γd pd pav pu K eb sp0 b wr sector bs_buf
-                    bs_disk m0 kq ({["virtio_disk"]} ∪ lks).
+                    bs_disk m0 kq ks ({["virtio_disk"]} ∪ lks).
   Proof.
     intros HK Hj Hjl Hbnz Hbelow.
     iIntros "#Htext #Hpinv #Hdinv #Hlk Hexit".
@@ -397,7 +397,7 @@ Section ProofVirtioDiskRwE.
     iIntros (CIDx Hsx M q np nr fl pk tr fr h m2 t pin)
             "%Hrh %Ha1 %Hok %Hpinr %Hal Hcg Hown Htc Hclm Hpc Htok Hbody Hclaim Hrm Hrt Hidx".
     destruct Hrh as (Hregs & Hhi).
-    set (V := DClaim b (vdrwd_slot kq b h wr sector (vdrwd_sldata wr bs_buf bs_disk))
+    set (V := DClaim b (vdrwd_slot kq ks b h wr sector (vdrwd_sldata wr bs_buf bs_disk))
                      (h, m2, t) pin).
     pose proof Hregs as Hregs'.
     destruct Hregs' as (Hsp & Hs0 & Hs3 & Hs6 & Hs7).
@@ -410,7 +410,7 @@ Section ProofVirtioDiskRwE.
     iPoseProof (rwi_1b0 with "Htext") as "Hi19c".
     (* ================= THE LOOP, first (it is used by both arms) ======= *)
     iAssert (vdrw_p5_loop CID γk γs j γd pd pav pu K eb sp0 b wr sector
-               bs_buf bs_disk h m2 t q pin m0 kq lks)%I with "[]" as "Hloop".
+               bs_buf bs_disk h m2 t q pin m0 kq ks lks)%I with "[]" as "Hloop".
     { iLöb as "IH". rewrite {2}/vdrw_p5_loop.
       iIntros (CIDlp Hslp M') "%Hinv Hcg Hown Htc Hclm Hpc Htok HR Hclaim Hrm Hrt Hidx
                     %HokL %HalL %HpinrL HexitL".
@@ -794,7 +794,8 @@ Section ProofVirtioDiskRwE.
                                 - virtio_base)%Z (mword_of_int 0 : mword 32) = Some v'
                 /\ virtio_isr_ok v'
                 /\ v_cfg v' = v_cfg v /\ v_seen v' = v_seen v
-                /\ v_used_idx v' = v_used_idx v /\ v_disk v' = v_disk v).
+                /\ v_used_idx v' = v_used_idx v /\ v_disk v' = v_disk v
+                /\ v_landed v' = v_landed v).
     { intros v Hvok. rewrite vdrwe_notify_off.
       apply (virtio_notify_write_ok v (mword_of_int 0 : mword 32));
         [ vm_compute; reflexivity | exact Hvok ]. }
